@prefix owl: <http://www.w3.org/2002/07/owl#> .
@prefix rdf: <http://www.w3.org/1999/02/22-rdf-syntax-ns#> .
@prefix xml: <http://www.w3.org/XML/1998/namespace> .
@prefix xsd: <http://www.w3.org/2001/XMLSchema#> .
@prefix rdfs: <http://www.w3.org/2000/01/rdf-schema#> .
@prefix swrl: <http://www.w3.org/2003/11/swrl#> .
@prefix swrlb: <http://www.w3.org/2003/11/swrlb#> .
@prefix spin:    <http://spinrdf.org/spin#> .
@prefix spl:     <http://spinrdf.org/spl#> .
@prefix LLM4BI: <http://www.foo.bar/LLM4BI/ontologies/LLM4BI#> .
@base <http://www.foo.bar/LLM4BI/ontologies/LLM4BI> .

<http://www.foo.bar/LLM4BI/ontologies/LLM4BI> rdf:type owl:Ontology .


LLM4BI:BIObject rdf:type owl:Class ;
    rdfs:comment "Represents an entity within the Dimensional Fact Model schema" .

LLM4BI:Fact rdfs:subClassOf LLM4BI:BIObject .

LLM4BI:ConformedHierarchyRoot rdfs:subClassOf LLM4BI:BIObject ;
    rdfs:comment "Represent the root attribute of a conformed hierarchy" .

LLM4BI:ConformedAttribute rdfs:subClassOf LLM4BI:BIObject ;
    rdfs:comment "Defines an attribute that is shared across multiple dimensions or fact tables and maintains the same meaning, domain of values, and granularity in all contexts where it appears." .

LLM4BI:Measure rdfs:subClassOf LLM4BI:BIObject .

LLM4BI:Attribute  rdfs:subClassOf LLM4BI:BIObject .

LLM4BI:Arc a owl:ObjectProperty ;
  rdfs:domain LLM4BI:BIObject ;
  rdfs:range  LLM4BI:BIObject ;
  rdfs:comment "An arc connecting entities within a Dimensional Fact Model schema. In presence of an arc from A to B, the user can roll-up from A to B." ; 
  rdfs:label "" .

LLM4BI:RollUpArc a owl:ObjectProperty ;
  rdfs:subPropertyOf LLM4BI:Arc ;
  rdfs:domain LLM4BI:BIObject ;
  rdfs:range  LLM4BI:BIObject ;
  rdfs:comment "Represents a functional dependency between two attributes connected by a many-to-one relationship (e.g., if one product belongs to one type, there is an arc from product to the type attribute)." ; 
  rdfs:label "" .

LLM4BI:MultipleArc a owl:ObjectProperty ;
    rdfs:subPropertyOf LLM4BI:Arc ;
    rdfs:comment "Represents a many-to-many-relationship between two attributes (e.g., if one book has several authors and an author writes several books, there is a multiple arc between author and book)" ;
    rdfs:label "MultipleArc" .

LLM4BI:OptionalArc a owl:ObjectProperty ;
    rdfs:subPropertyOf LLM4BI:Arc ;
    rdfs:comment "Defines an optional arc between two entities (e.g.,  there is an optional arc from Product to Diet_Y/N because Diet_Y/N has no value for some product)" ;
    rdfs:label "OptionalArc" .

LLM4BI:LogicalName a owl:DataTypeProperty ;
  rdfs:domain LLM4BI:BIObject ;
  rdfs:comment "Defines the name of the attribute within the logical schema" ;
  rdfs:range xsd:string .

LLM4BI:SampleValues a owl:DataTypeProperty ;
  rdfs:domain LLM4BI:BIObject ;
  rdfs:comment "Defines a set of values for an attribute/measure" ;
  rdfs:range xsd:string .

LLM4BI:AggregationOperator a owl:DataTypeProperty ;
  rdfs:domain LLM4BI:Measure ;
  rdfs:comment "Defines the operator that can be used to aggregate a measure along one hierarchy (e.g., SUM,AVG,MIN,MAX)" ;
  rdfs:range xsd:string .

LLM4BI:Description a owl:DataTypeProperty ;
  rdfs:domain LLM4BI:BIObject ;
  rdfs:comment "A description for what an entity represents in the business logic" ;
  rdfs:range xsd:string .

LLM4BI:Notes a owl:DataTypeProperty ;
  rdfs:domain LLM4BI:BIObject ;
  rdfs:comment "Additional notes regarding an entity." ;
  rdfs:range xsd:string .

LLM4BI:isConvergence a owl:DataTypeProperty ;
  rdfs:domain LLM4BI:BIObject ;
  rdfs:comment "In a convergence, two attributes are connected by two or more distinct directed paths of arcs, and each of them still represents a functional dependency." ;
  rdfs:range xsd:boolean .

LLM4BI:isShared a owl:DataTypeProperty ;
  rdfs:domain LLM4BI:BIObject ;
  rdfs:comment "A shared hierarchy denotes that an attribute (part of a hierarchy) is replicated two or more times within a fact schema." ;
  rdfs:range xsd:boolean .

LLM4BI:isCrossDimensional a owl:DataTypeProperty ;
  rdfs:domain LLM4BI:BIObject ;
  rdfs:comment "A cross-dimensional attribute is a dimensional or descriptive attribute whose value is defined by the combination of two or more dimensional attributes, possibly belonging to different hierarchies." ;
  rdfs:range xsd:boolean .

LLM4BI:isDescriptive a owl:DataTypeProperty ;
  rdfs:domain LLM4BI:BIObject ;
  rdfs:comment "A descriptive attribute stores additional information about another attribute and is not used for aggregation because it has a dense domain and/or it is the child of a one-to-one association." ;
  rdfs:range xsd:boolean .